src/Parsers/ContextFreeGrammar/Fix/Correct.v
@@ -1,7 +1,5 @@
-Require Import Coq.Classes.Morphisms.
 Require Import Fiat.Parsers.BaseTypes.
 Require Import Fiat.Parsers.Splitters.RDPList.
-Require Import Fiat.Parsers.ContextFreeGrammar.Core.
 Require Import Fiat.Parsers.ContextFreeGrammar.PreNotations.
 Require Import Fiat.Parsers.ContextFreeGrammar.Carriers.
 Require Import Fiat.Parsers.ContextFreeGrammar.Fix.Fix.
