src/Parsers/Refinement/BinOpBrackets/ParenBalancedGrammar.v
@@ -5,9 +5,7 @@ Require Import Fiat.Parsers.Reachable.ParenBalanced.Core.
 Require Import Fiat.Parsers.ContextFreeGrammar.Core.
 Require Import Fiat.Parsers.ContextFreeGrammar.PreNotations.
 Require Import Fiat.Parsers.BaseTypes.
-Require Import Fiat.Parsers.StringLike.Core.
 Require Import Fiat.Parsers.StringLike.Properties.
-Require Import Fiat.Parsers.ContextFreeGrammar.Fold.
 Require Import Fiat.Common.Equality.
 Require Import Fiat.Common.List.Operations.
 Require Import Fiat.Common.
