src/Parsers/Refinement/DisjointRules.v
@@ -1,15 +1,10 @@
 (** Refinement rules for disjoint rules *)
-Require Import Coq.Lists.List.
 Require Import Fiat.Parsers.Refinement.PreTactics.
 Require Import Fiat.Computation.Refinements.General.
 Require Import Fiat.Parsers.StringLike.Properties.
-Require Import Fiat.Parsers.StringLike.FirstCharSuchThat.
 Require Import Fiat.Parsers.StringLike.FirstChar.
-Require Import Fiat.Common.
 Require Import Fiat.Common.Equality.
 Require Import Fiat.Common.List.Operations.
-Require Import Fiat.Parsers.Splitters.RDPList.
-Require Import Fiat.Parsers.BaseTypes.
 Require Import Fiat.Parsers.ContextFreeGrammar.ValidReflective.
 Require Import Fiat.Parsers.Refinement.DisjointLemmas.
 Require Import Fiat.Parsers.ParserInterface.
