src/Parsers/Refinement/PossibleTerminalsSets.v
@@ -3,14 +3,12 @@ Require Import Coq.Classes.Morphisms.
 Require Import Fiat.Parsers.StringLike.FirstChar Fiat.Parsers.StringLike.LastChar Fiat.Parsers.StringLike.ForallChars.
 Require Import Fiat.Parsers.ContextFreeGrammar.Core.
 Require Import Fiat.Parsers.ContextFreeGrammar.PreNotations.
-Require Import Fiat.Parsers.StringLike.Core.
 Require Import Fiat.Parsers.StringLike.Properties.
 Require Import Fiat.Parsers.Splitters.RDPList.
 Require Import Fiat.Parsers.BaseTypes.
 Require Import Fiat.Parsers.ContextFreeGrammar.Fix.FromAbstractInterpretationDefinitions.
 Require Import Fiat.Parsers.ContextFreeGrammar.Fix.Fix.
 Require Import Fiat.Parsers.ContextFreeGrammar.Fix.AsciiLattice.
-Require Import Fiat.Parsers.ContextFreeGrammar.Fix.Prod.
 Require Import Fiat.Parsers.ContextFreeGrammar.Fix.ProdAbstractInterpretationDefinitions.
 Require Import Fiat.Parsers.ContextFreeGrammar.Fix.FromAbstractInterpretation.
 Require Import Fiat.Parsers.Refinement.EmptyLemmas.
